CertifyingDatalog/Basic.lean
@@ -1,0 +1,17 @@
+import Mathlib.Data.Set.Basic
+
+
+def List.toSet {A: Type} (l: List A): Set A :=
+  match l with
+  | [] => ∅
+  | hd::tl => {hd} ∪ tl.toSet
+
+lemma List.toSet_mem {A: Type} (a:A) (l: List A): a ∈ l ↔ a ∈ l.toSet := by
+  induction l with
+  | nil =>
+    unfold List.toSet
+    simp
+  | cons hd tl ih =>
+    unfold List.toSet
+    simp
+    rw [ih]
